Try new cx

src/defs/var.lean
@@ -13,172 +13,60 @@ structure cx_elem (t: Type): Type :=
 def ne_var {t: Type} (a b: cx_elem t): Prop :=
   a.x ≠ b.x
 
+structure cx (t: Type): Type :=
+  (entries: set (cx_elem t))
+  (nodupkeys:
+    ∀ (e e' ∈ entries),
+    e ≠ e' ->
+    ne_var e e'
+  )
+
+def cx.empty {t: Type}: cx t :=
+  cx.mk ∅ begin
+    intros a b a_in,
+    exfalso,
+    exact a_in,
+  end
+
+def cx.lookup {t: Type} (Γ: cx t) (x: var) (v: t): Prop :=
+  (cx_elem.mk x v ∈ Γ.entries)
+
+def cx.insert {t: Type} (Γ: cx t) (x: var) (v: t): cx t :=
+cx.mk ({cx_elem.mk x v} ∪ { e ∈ Γ.entries | cx_elem.x e ≠ x }) begin
+  intros e e' e_in e'_in e_ne,
+  cases e_in,
+  cases e_in,
+  cases e'_in,
+  cases e'_in,
+  rw symm e'_in at e_in,
+  exfalso,
+  exact e_ne e_in,
+  exfalso,
+  exact e'_in,
+  cases e'_in,
+  simp [ne_var],
+  rw e_in,
+  simp,
+  let h := fun hm, e'_in_right (symm hm),
+  exact h,
+  exfalso,
+  exact e_in,
+  cases e_in,
+  cases e'_in,
+  cases e'_in,
+  simp [ne_var],
+  rw e'_in,
+  simp,
+  exact e_in_right,
+  exfalso,
+  exact e'_in,
+  cases e'_in,
+  exact Γ.nodupkeys e e' e_in_left e'_in_left e_ne,
+end
+
 instance {t: Type}: is_symm (cx_elem t) ne_var := is_symm.mk
 begin
   intros a b ab,
   simp [ne_var] at *,
   exact ne.symm ab,
-end
-
-def cx_elem_lt {t: Type} [decidable_linear_order t] (a b: cx_elem t): Prop :=
-  if a.x = b.x then a.v < b.v else a.x < b.x
-
-def cx_elem_le {t: Type} [decidable_linear_order t] (a b: cx_elem t): Prop :=
-  if a.x = b.x then a.v ≤ b.v else a.x ≤ b.x
-
-instance cx_elem_decidable_linear_order {t: Type} [decidable_linear_order t]:
-decidable_linear_order (cx_elem t) :=
-decidable_linear_order.mk
-cx_elem_le
-cx_elem_lt
-begin
-  intro a,
-  simp,
-  simp [cx_elem_le],
-end
-begin
-  intros a b c ab bc,
-  simp at *,
-  simp [cx_elem_le] at *,
-  by_cases a.x = b.x,
-  simp [h] at ab,
-  by_cases h_1: b.x = c.x,
-  simp [h_1] at bc,
-  rw h_1 at h,
-  simp [h],
-  exact le_trans ab bc,
-  simp [h_1] at bc,
-  rw symm h at h_1 bc,
-  simp [h_1],
-  exact bc,
-  simp [h] at ab,
-  by_cases h_1: b.x = c.x,
-  simp [h_1] at bc,
-  rw h_1 at h ab,
-  simp [h],
-  exact ab,
-  simp [h_1] at bc,
-  let ab' := lt_of_le_of_ne ab h,
-  let bc' := lt_of_le_of_ne bc h_1,
-  let ac := lt_trans ab' bc',
-  simp [ne_of_lt ac],
-  exact le_trans ab bc,
-end
-begin
-  intros a b,
-  simp,
-  simp [cx_elem_lt],
-  simp [cx_elem_le],
-  split,
-  intro ab,
-  by_cases a.x = b.x,
-  simp [h] at ab ⊢,
-  exact iff.elim_left lt_iff_le_not_le ab,
-  simp [h] at ab ⊢,
-  let h' := fun x, h (symm x),
-  simp [h'],
-  exact iff.elim_left lt_iff_le_not_le ab,
-  intro ab,
-  by_cases a.x = b.x,
-  simp [h] at ab ⊢,
-  exact iff.elim_right lt_iff_le_not_le ab,
-  simp [h] at ab ⊢,
-  let h' := fun x, h (symm x),
-  simp [h'] at ab,
-  exact iff.elim_right lt_iff_le_not_le ab,
-end
-begin
-  intros a b ab ba,
-  simp [(≤)] at ab ba,
-  simp [cx_elem_le] at ab ba,
-  cases a,
-  cases b,
-  simp at ab ba ⊢,
-  by_cases a_x = b_x,
-  simp [h] at ab ba,
-  let eq_v := le_antisymm ab ba,
-  split,
-  exact h,
-  exact eq_v,
-  simp [h] at ab,
-  let h' := fun x, h (symm x),
-  simp [h'] at ba,
-  exfalso,
-  exact h (le_antisymm ab ba),
-end
-begin
-  intros a b,
-  simp [(≤)],
-  simp [preorder.le],
-  simp [cx_elem_le],
-  by_cases a.x = b.x,
-  simp [h],
-  exact le_total a.v b.v,
-  simp [h],
-  let h' := fun x, h (symm x),
-  simp [h'],
-  exact le_total a.x b.x,
-end
-begin
-  intros a b,
-  simp [(≤)],
-  simp [preorder.le],
-  simp [partial_order.le],
-  simp [cx_elem_le],
-  by_cases a.x = b.x,
-  simp [h],
-  exact decidable_linear_order.decidable_le t a.v b.v,
-  simp [h],
-  exact nat.decidable_le a.x b.x,
-end
-(cx_elem.decidable_eq t)
-begin
-  intros a b,
-  simp [(<)],
-  simp [preorder.lt],
-  simp [partial_order.lt],
-  simp [cx_elem_lt],
-  by_cases a.x = b.x,
-  simp [h],
-  exact decidable_linear_order.decidable_lt t a.v b.v,
-  simp [h],
-  exact nat.decidable_lt a.x b.x,
-end
-
-structure cx (t: Type) [decidable_linear_order t]: Type :=
-  (entries: list (cx_elem t))
-  (nodupkeys: pairwise ne_var entries)
-  (sorted: sorted entries)
-
-def cx.empty {t: Type} [decidable_linear_order t]: cx t :=
-  cx.mk [] (pairwise.nil ne_var) (pairwise.nil (≤))
-
-def cx.lookup {t: Type} [decidable_linear_order t] (Γ: cx t) (x: var): option t :=
-begin
-  cases Γ,
-  induction Γ_entries,
-  exact none,
-  exact (if x = Γ_entries_hd.x then
-    some Γ_entries_hd.v
-  else
-    -- avoid weird 'can only eliminate into Prop' error when trying to use cases
-    Γ_entries_ih
-      (pairwise_inversion Γ_nodupkeys)
-      (pairwise_inversion Γ_sorted)
-  ),
-end
-
-def cx.insert {t: Type} [decidable_linear_order t] (Γ: cx t) (x: var) (v: t): cx t :=
-begin
-  cases Γ,
-  let elem := cx_elem.mk x v,
-  let p: cx_elem t -> Prop := fun a, x ≠ a.x,
-  let entries' := insertion_sort (elem :: list.filter p Γ_entries),
-  let f := fun (a: cx_elem t), fun (b: a ∈ list.filter p Γ_entries),
-    (iff.elim_right filter_spec b).right,
-  let nodupkeys' := insertion_sort_pairwise (@pairwise.cons
-    (cx_elem t) ne_var elem (list.filter p Γ_entries) f
-    (filter_pairwise p Γ_nodupkeys)),
-  let sorted' := insertion_sort_spec (elem :: list.filter p Γ_entries),
-  exact cx.mk entries' nodupkeys' sorted',
 end
