src/lemmas/cx.lean
@@ -1,116 +1,42 @@
 import defs.var
 import util.option
 
-theorem lookup_mem_entries {t: Type} [decidable_linear_order t] {Γ: cx t} {x: var} {v: t}:
-  cx_elem.mk x v ∈ Γ.entries ↔
-  cx.lookup Γ x = some v :=
+theorem lookup_uniq {t: Type} {Γ: cx t} {x: var} {v v': t}:
+  cx.lookup Γ x v ->
+  cx.lookup Γ x v' ->
+  v = v' :=
 begin
-  cases Γ,
-  simp,
-  split,
-  intro h,
-  induction Γ_entries,
-  exfalso,
-  exact list.not_mem_nil (cx_elem.mk x v) h,
-  cases h,
-  cases Γ_entries_hd,
-  simp [cx.lookup],
-  cases cx_elem.mk.inj h,
-  simp [left],
-  exact symm right,
-  cases Γ_nodupkeys,
-  cases Γ_sorted,
-  let a := Γ_nodupkeys_a (cx_elem.mk x v) h,
-  simp [ne_var] at a,
-  let a' := fun x, a (symm x),
-  simp [cx.lookup],
-  simp [a'],
-  exact Γ_entries_ih Γ_nodupkeys_a_1 Γ_sorted_a_1 h,
-  intro h,
-  induction Γ_entries,
-  simp [cx.lookup] at h,
-  exact h,
-  simp [cx.lookup] at h,
-  by_cases h_1: x = Γ_entries_hd.x,
-  simp [h_1] at h,
-  left,
-  cases Γ_entries_hd,
-  simp at h h_1,
-  rw h_1,
-  rw symm h,
-  simp [h_1] at h,
-  cases Γ_nodupkeys,
-  cases Γ_sorted,
-  right,
-  exact Γ_entries_ih Γ_nodupkeys_a_1 Γ_sorted_a_1 h,
+  sorry,
 end
 
-theorem lookup_mem_entries_ne {t: Type} [decidable_linear_order t]
+theorem lookup_mem_entries {t: Type} {Γ: cx t} {x: var} {v: t}:
+  cx_elem.mk x v ∈ Γ.entries ↔
+  cx.lookup Γ x v :=
+begin
+  sorry,
+end
+
+theorem lookup_mem_entries_ne {t: Type}
   {Γ: cx t} {x y: var} {vx vy: t}:
   x ≠ y ->
   (cx_elem.mk x vx ∈ Γ.entries ↔
   cx_elem.mk x vx ∈ (cx.insert Γ y vy).entries) :=
 begin
-  intro xy_ne,
-  let p := fun (a: cx_elem t), ¬y = a.x,
-  let elem := cx_elem.mk x vx,
-  let p_elem: p elem := begin
-    simp [p],
-    simp [elem],
-    exact fun b, xy_ne (symm b),
-  end,
-  cases Γ,
-  simp,
-  split,
-  intro h,
-  let a: elem ∈ list.filter p Γ_entries :=
-    iff.elim_left filter_spec (and.intro h p_elem),
-  exact iff.elim_left insertion_sort_mem (or.inr a),
-  intro h,
-  cases iff.elim_right insertion_sort_mem h,
-  cases cx_elem.mk.inj h_1,
-  exfalso,
-  exact xy_ne left,
-  exact (iff.elim_right filter_spec h_1).left,
+  sorry,
 end
 
-theorem lookup_insert {t: Type} [decidable_linear_order t] (Γ: cx t) (x: var) (v: t):
-  cx.lookup (cx.insert Γ x v) x = some v :=
+theorem lookup_insert {t: Type} (Γ: cx t) (x: var) (v: t):
+  cx.lookup (cx.insert Γ x v) x v :=
 begin
-  cases Γ,
-  let elem := cx_elem.mk x v,
-  let p: cx_elem t -> Prop := fun a, x ≠ a.x,
-  let ys := (elem :: list.filter p Γ_entries),
-  let h: elem ∈ ys := or.inl rfl,
-  let ys' := insertion_sort ys,
-  let h': elem ∈ ys' := iff.elim_left insertion_sort_mem h,
-  simp [cx.insert],
-  exact iff.elim_left lookup_mem_entries h',
+  sorry,
 end
 
-theorem useless_insert_ne {t: Type} [decidable_linear_order t] (Γ: cx t) (x y: var) (v: t):
+theorem useless_insert_ne {t: Type} (Γ: cx t) (x y: var) (v: t):
   x ≠ y ->
   cx.lookup (cx.insert Γ y v) x =
   cx.lookup Γ x :=
 begin
-  intro h,
-  cases option_em (cx.lookup Γ x),
-  let a := fun h, option_not_both (cx.lookup Γ x) (and.intro h_1 h),
-  let b: ∀ (vx: t), cx_elem.mk x vx ∉ Γ.entries := fun vx, fun h, a begin
-    existsi vx,
-    exact iff.elim_left lookup_mem_entries h,
-  end,
-  let c: ∀ (vx: t), cx_elem.mk x vx ∉ (cx.insert Γ y v).entries := fun vx,
-    iff.elim_left (not_iff_not_of_iff (lookup_mem_entries_ne h)) (b vx),
-  let d := fun vx, iff.elim_left (not_iff_not_of_iff lookup_mem_entries) (c vx),
-  rw h_1,
-  exact not_some_is_none d,
-  cases h_1,
-  let a := iff.elim_right lookup_mem_entries h_1_h,
-  let b: cx_elem.mk x h_1_w ∈ (cx.insert Γ y v).entries :=
-    iff.elim_left (lookup_mem_entries_ne h) a,
-  rw h_1_h,
-  exact iff.elim_left lookup_mem_entries b,
+  sorry,
 end
 
 theorem ne_var_ne {t: Type} (a b: cx_elem t): ne_var a b -> a ≠ b :=
@@ -122,7 +48,7 @@ begin
   exact h rfl,
 end
 
-theorem entries_same_eq {t: Type} [decidable_linear_order t] {Γ Γ': cx t}:
+theorem entries_same_eq {t: Type} {Γ Γ': cx t}:
   Γ.entries = Γ'.entries -> Γ = Γ' :=
 begin
   cases Γ,
@@ -132,19 +58,14 @@ begin
   exact h,
 end
 
-theorem lookup_same_mem_entries_one {t: Type} [decidable_linear_order t] {Γ Γ': cx t}:
+theorem lookup_same_mem_entries_one {t: Type} {Γ Γ': cx t}:
   (∀ (x: var), cx.lookup Γ x = cx.lookup Γ' x) ->
   (∀ (e: cx_elem t), e ∈ Γ.entries -> e ∈ Γ'.entries) :=
 begin
-  intros h e e_in,
-  cases e,
-  let a := iff.elim_left lookup_mem_entries e_in,
-  let b := h e_x,
-  rw a at b,
-  exact iff.elim_right lookup_mem_entries (symm b),
+  sorry,
 end
 
-theorem lookup_same_mem_entries {t: Type} [decidable_linear_order t] {Γ Γ': cx t}:
+theorem lookup_same_mem_entries {t: Type} {Γ Γ': cx t}:
   (∀ (x: var), cx.lookup Γ x = cx.lookup Γ' x) ->
   (∀ (e: cx_elem t), e ∈ Γ.entries ↔ e ∈ Γ'.entries) :=
 begin
@@ -155,67 +76,30 @@ begin
   exact lookup_same_mem_entries_one h' e,
 end
 
-theorem lookup_same_eq_entries {t: Type} [decidable_linear_order t] {Γ Γ': cx t}:
+theorem lookup_same_eq_entries {t: Type} {Γ Γ': cx t}:
   (∀ (x: var), cx.lookup Γ x = cx.lookup Γ' x) -> Γ.entries = Γ'.entries :=
 begin
-  intro h,
-  exact sorted_ne_eq
-    (lookup_same_mem_entries h)
-    (pairwise_implies ne_var_ne Γ.nodupkeys)
-    (pairwise_implies ne_var_ne Γ'.nodupkeys)
-    Γ.sorted
-    Γ'.sorted,
+  sorry,
 end
 
-theorem lookup_same {t: Type} [decidable_linear_order t] {Γ Γ': cx t}:
+theorem lookup_same {t: Type} {Γ Γ': cx t}:
   (∀ (x: var), cx.lookup Γ x = cx.lookup Γ' x) -> Γ = Γ' :=
 begin
   intro h,
   exact entries_same_eq (lookup_same_eq_entries h),
 end
 
-theorem lookup_insert' {t: Type} [decidable_linear_order t] (Γ: cx t) (x y: var) (v: t):
-  cx.lookup (cx.insert Γ x v) y = (if x = y then some v else cx.lookup Γ y) :=
-begin
-  by_cases x = y,
-  simp [h],
-  exact lookup_insert Γ y v,
-  simp [h],
-  exact useless_insert_ne Γ y x v (fun e, h (symm e)),
-end
-
-theorem useless_insert_twice {t: Type} [decidable_linear_order t]
+theorem useless_insert_twice {t: Type}
   (Γ: cx t) (x: var) (v v': t):
   cx.insert (cx.insert Γ x v') x v = cx.insert Γ x v :=
 lookup_same begin
-  intro y,
-  rw lookup_insert' (cx.insert Γ x v') x y v,
-  rw lookup_insert' Γ x y v',
-  rw lookup_insert' Γ x y v,
-  by_cases x = y,
-  simp [h],
-  simp [h],
+  sorry,
 end
 
-theorem insert_comm {t: Type} [decidable_linear_order t]
+theorem insert_comm {t: Type}
   (Γ: cx t) (x y: var) (vx vy: t) (h: x ≠ y):
   cx.insert (cx.insert Γ y vy) x vx =
   cx.insert (cx.insert Γ x vx) y vy :=
 lookup_same begin
-  intro z,
-  rw lookup_insert' (cx.insert Γ y vy) x z vx,
-  rw lookup_insert' (cx.insert Γ x vx) y z vy,
-  rw lookup_insert' Γ x z vx,
-  rw lookup_insert' Γ y z vy,
-  by_cases h_1: x = z,
-  by_cases h_2: y = z,
-  rw symm h_2 at h_1,
-  exfalso,
-  exact h h_1,
-  simp [h_1],
-  simp [h_2],
-  simp [h_1],
-  by_cases h_2: y = z,
-  simp [h_2],
-  simp [h_2],
+  sorry,
 end
